cleaned up spec mono proof

thm2_TEMP.thy
@@ -66,17 +66,15 @@ lemma norm_spec_mono:
   by (smt (verit, ccfv_SIG) One_nat_def assms(3) mono_denormI mult_left_mono)
   
 (*Interval definition: *)
-definition int :: "(real \<times> real) list" where
-"int = [ ((normI 1 (inRanges(1).1)), ((normI 1 (inRanges(1).2)))), 
+definition normRanges :: "(real \<times> real) list" where
+"normRanges = [ ((normI 1 (inRanges(1).1)), ((normI 1 (inRanges(1).2)))), 
          ((normI 2 (inRanges(2).1)), ((normI 2 (inRanges(2).2)))) ]"
-term "#int"
 
-
-(*Using FST for MIN and SND for MAX, when encoding the intervals. *)
-term "fst(int(1))"
-term "fst(int(2))"
-term "snd(int(1))"
-term "snd(int(2))"
+(*Using FST for MIN and SND for MAX, when encoding the normRangeservals. *)
+term "fst(normRanges(1))"
+term "fst(normRanges(2))"
+term "snd(normRanges(1))"
+term "snd(normRanges(2))"
 
 (*Abbreviation for readability, referring to the f_ann as annout 2 1 to correspond 
 to the last layer of our example: *)
@@ -85,58 +83,62 @@ abbreviation "f_ann x y \<equiv> annout 2 1 [x,y]"
 term "f_ann 0 0"
 
 lemma spec_mono_ann:
-  fixes x_1 x_2 y_1 y_2 :: real and
+  fixes x_1 x_2 :: real and
         S :: "real \<Rightarrow> real \<Rightarrow> real" and 
         f :: "real \<Rightarrow> real \<Rightarrow> real" 
   assumes 
-          "fst(int(1)) \<le> x_1 \<and> x_1 \<le> snd(int(1))" and 
-          "fst(int(2)) \<le> x_2 \<and> x_2 \<le> snd(int(2))" and 
+          "fst(normRanges(1)) \<le> x_1 \<and> x_1 \<le> snd(normRanges(1))" and 
+          "fst(normRanges(2)) \<le> x_2 \<and> x_2 \<le> snd(normRanges(2))" and 
           "(snd(outRanges ! 0) > fst(outRanges ! 0) \<and> snd(annRange) > fst(annRange))" and
           "\<epsilon> \<ge> 0" and 
-          "f x_1 x_2 \<le> normO 1 (S (fst(int(1))) (fst(int(2))) + \<epsilon>)
-               \<and> f x_1 x_2 \<ge> normO 1 (S (snd(int(1))) (snd(int(2))) - \<epsilon>) 
-              " and 
           (*Monotonicity property for our specification function: *)
           "\<forall> x_1 x_2 y_1 y_2 :: real. x_1 \<le> y_1 \<and> x_2 \<le> y_2 \<longrightarrow> S x_1 x_2 \<le> S y_1 y_2"
         shows "
+              f x_1 x_2 \<le> normO 1 (S (fst(normRanges(1))) (fst(normRanges(2))) + \<epsilon>)
+               \<and> f x_1 x_2 \<ge> normO 1 (S (snd(normRanges(1))) (snd(normRanges(2))) - \<epsilon>) 
+              \<Longrightarrow>
                f x_1 x_2 \<ge> (normO 1 (S (x_1) (x_2) - \<epsilon>)) \<and>
                f x_1 x_2 \<le> (normO 1 (S (x_1) (x_2) + \<epsilon>)) 
                 "
 proof (rule conjI)
-  have 1: "f x_1 x_2 \<le> normO 1 (S (fst(int(1))) (fst(int(2))) + \<epsilon>)" using assms by simp 
-  have 2: "f x_1 x_2 \<ge> normO 1 (S (snd(int(1))) (snd(int(2))) - \<epsilon>)" using assms by simp
+  assume a1:"f x_1 x_2 \<le> normO 1 (S (fst(normRanges(1))) (fst(normRanges(2))) + \<epsilon>)
+               \<and> f x_1 x_2 \<ge> normO 1 (S (snd(normRanges(1))) (snd(normRanges(2))) - \<epsilon>) 
+              "
+
+  have 1: "f x_1 x_2 \<le> normO 1 (S (fst(normRanges(1))) (fst(normRanges(2))) + \<epsilon>)" using a1 by simp 
+  have 2: "f x_1 x_2 \<ge> normO 1 (S (snd(normRanges(1))) (snd(normRanges(2))) - \<epsilon>)" using a1 by simp
 
   (*GOAL 1: first conjunct of the goal: *)
-  from assms(1) assms(2) have "x_1 \<ge> fst(int(1)) \<and> x_2 \<ge> fst(int(2))" by simp
+  from assms(1) assms(2) have "x_1 \<ge> fst(normRanges(1)) \<and> x_2 \<ge> fst(normRanges(2))" by simp
   have "... \<longrightarrow> 
-        (S x_1 x_2) \<ge> (S (fst(int(1))) (fst(int(2))))" 
+        (S x_1 x_2) \<ge> (S (fst(normRanges(1))) (fst(normRanges(2))))" 
     using assms by simp
   have "... \<longrightarrow> 
-        (S x_1 x_2) + \<epsilon> \<ge> (S (fst(int(1))) (fst(int(2)))) + \<epsilon>"
+        (S x_1 x_2) + \<epsilon> \<ge> (S (fst(normRanges(1))) (fst(normRanges(2)))) + \<epsilon>"
     by simp
   have c1:"... \<longrightarrow> 
-        normO 1 ((S x_1 x_2) + \<epsilon>) \<ge> normO 1 ((S (fst(int(1))) (fst(int(2)))) + \<epsilon>)"
+        normO 1 ((S x_1 x_2) + \<epsilon>) \<ge> normO 1 ((S (fst(normRanges(1))) (fst(normRanges(2)))) + \<epsilon>)"
     using assms 
     apply (simp add: mono_normO)
     by (smt (verit, ccfv_SIG) diff_Suc_1 mono_normO)
   from 1 c1 show "f x_1 x_2 \<le> normO 1 ((S x_1 x_2) + \<epsilon>)"
-    using \<open>fst (thm2_TEMP.int(1)\<^sub>s) \<le> x_1 \<and> fst (thm2_TEMP.int(2)\<^sub>s) \<le> x_2\<close> \<open>fst (thm2_TEMP.int(2)\<^sub>s) \<le> x_2 \<longrightarrow> S (fst (thm2_TEMP.int(1)\<^sub>s)) (fst (thm2_TEMP.int(2)\<^sub>s)) \<le> S x_1 x_2\<close> by argo
+    using \<open>fst (thm2_TEMP.normRanges(1)\<^sub>s) \<le> x_1 \<and> fst (thm2_TEMP.normRanges(2)\<^sub>s) \<le> x_2\<close> \<open>fst (thm2_TEMP.normRanges(2)\<^sub>s) \<le> x_2 \<longrightarrow> S (fst (thm2_TEMP.normRanges(1)\<^sub>s)) (fst (thm2_TEMP.normRanges(2)\<^sub>s)) \<le> S x_1 x_2\<close> by argo
     
   (*Goal 2: second cojunct of the goal: *)
-  from assms(1) assms(2) have "x_1 \<le> snd(int(1)) \<and> x_2 \<le> snd(int(2))" by simp
+  from assms(1) assms(2) have "x_1 \<le> snd(normRanges(1)) \<and> x_2 \<le> snd(normRanges(2))" by simp
   have "... \<longrightarrow> 
-        (S x_1 x_2) \<le> (S (snd(int(1))) (snd(int(2))))" 
+        (S x_1 x_2) \<le> (S (snd(normRanges(1))) (snd(normRanges(2))))" 
     using assms by simp
   have "... \<longrightarrow> 
-        (S x_1 x_2) - \<epsilon> \<le> (S (snd(int(1))) (snd(int(2)))) - \<epsilon>"
+        (S x_1 x_2) - \<epsilon> \<le> (S (snd(normRanges(1))) (snd(normRanges(2)))) - \<epsilon>"
     by simp
   have c2: "... \<longrightarrow> 
-        normO 1 ((S x_1 x_2) - \<epsilon>) \<le> normO 1 ((S (snd(int(1))) (snd(int(2)))) - \<epsilon>)"
+        normO 1 ((S x_1 x_2) - \<epsilon>) \<le> normO 1 ((S (snd(normRanges(1))) (snd(normRanges(2)))) - \<epsilon>)"
     using assms 
     apply (simp add: mono_normO)
     by (smt (verit, ccfv_SIG) diff_Suc_1 mono_normO)
   from 2 c2 show "f x_1 x_2 \<ge> (normO 1 (S (x_1) (x_2) - \<epsilon>))"
-    using \<open>x_1 \<le> snd (thm2_TEMP.int(1)\<^sub>s) \<and> x_2 \<le> snd (thm2_TEMP.int(2)\<^sub>s)\<close> \<open>x_2 \<le> snd (thm2_TEMP.int(2)\<^sub>s) \<longrightarrow> S x_1 x_2 \<le> S (snd (thm2_TEMP.int(1)\<^sub>s)) (snd (thm2_TEMP.int(2)\<^sub>s))\<close> by linarith
+    using \<open>x_1 \<le> snd (thm2_TEMP.normRanges(1)\<^sub>s) \<and> x_2 \<le> snd (thm2_TEMP.normRanges(2)\<^sub>s)\<close> \<open>x_2 \<le> snd (thm2_TEMP.normRanges(2)\<^sub>s) \<longrightarrow> S x_1 x_2 \<le> S (snd (thm2_TEMP.normRanges(1)\<^sub>s)) (snd (thm2_TEMP.normRanges(2)\<^sub>s))\<close> by linarith
 qed
 
 (*Marabou combined results: *)
@@ -152,21 +154,21 @@ term "inRanges"
 (*The idea is, we have 2 facts that are evaluated expressions, that we use 
 to show the truth of symbolic expressions, with constant definitions
 
-That we can then reason about the fst int, etc, algebriacally within Isabelle.
+That we can then reason about the fst normRanges, etc, algebriacally within Isabelle.
 
 But we only prove the evaluated expressions, it only works if we instantiate 
 the constants but this is fine. *)
 
 (*Evaluated expressions, for Marabou translation: *)
-value "fst(int(1))"
-value "snd(int(1))"
-value "fst(int(2))"
-value "snd(int(2))"
-value "normO 1 ((P * denormI 1 (fst(int(1))) + (D * denormI 2 (fst(int(2)))) ) + \<epsilon>)"
-value "normO 1 ((P * denormI 1 (snd(int(1))) + (D * denormI 2 (snd(int(2)))) ) - \<epsilon>)"
+value "fst(normRanges(1))"
+value "snd(normRanges(1))"
+value "fst(normRanges(2))"
+value "snd(normRanges(2))"
+value "normO 1 ((P * denormI 1 (fst(normRanges(1))) + (D * denormI 2 (fst(normRanges(2)))) ) + \<epsilon>)"
+value "normO 1 ((P * denormI 1 (snd(normRanges(1))) + (D * denormI 2 (snd(normRanges(2)))) ) - \<epsilon>)"
 
 (*We need to have a strategy for the splits, automatically. 
-we already have int, meaningless without the splits. 
+we already have normRanges, meaningless without the splits. 
 
 We need it to be automatic, automated evaluation as well. 
 
@@ -176,16 +178,16 @@ evaluation, we don't want this. evaluating, partial evaluation ?
 
 
 
-lemma marabou_combined_results: 
+lemma marabou_results: 
   fixes x1 x2 :: real
-  assumes "x1 \<ge> fst(int(1)) \<and> 
-          x1 \<le> snd(int(1)) \<and>
-          x2 \<ge> fst(int(2)) \<and>
-          x2 \<le> snd(int(2))"
+  assumes "x1 \<ge> fst(normRanges(1)) \<and> 
+          x1 \<le> snd(normRanges(1)) \<and>
+          x2 \<ge> fst(normRanges(2)) \<and>
+          x2 \<le> snd(normRanges(2))"
   shows "
-          \<not> f_ann x1 x2 \<ge> normO 1 ((P * denormI 1 (fst(int(1))) + (D * denormI 2 (fst(int(2)))) ) + \<epsilon>)
+          \<not> f_ann x1 x2 \<ge> normO 1 ((P * denormI 1 (fst(normRanges(1))) + (D * denormI 2 (fst(normRanges(2)))) ) + \<epsilon>)
            \<and>           
-          \<not> f_ann x1 x2 \<le> normO 1 ((P * denormI 1 (snd(int(1))) + (D * denormI 2 (snd(int(2)))) ) - \<epsilon>)
+          \<not> f_ann x1 x2 \<le> normO 1 ((P * denormI 1 (snd(normRanges(1))) + (D * denormI 2 (snd(normRanges(2)))) ) - \<epsilon>)
 " 
 proof - 
   have 1: "x1 \<ge> 0 \<and> 
@@ -203,14 +205,14 @@ proof -
         " sorry
   
   from 1 2 show "?thesis"
-    using assms unfolding int_def P_def D_def inRanges_def annRange_def normI_def norm_def int_def
+    using assms unfolding normRanges_def P_def D_def inRanges_def annRange_def normI_def norm_def normRanges_def
 denormI_def normO_def outRanges_def \<epsilon>_def
     apply (simp)
     done    
 qed
 
 
-(*Rewrite this using our interval definitions, and f_ann, and spec_f. *)
+(*Rewrite this using our normRangeserval definitions, and f_ann, and spec_f. *)
 theorem controller_conformance:
   fixes x_1 x_2 :: real
   assumes 
@@ -236,7 +238,7 @@ shows " (conf_sin \<epsilon> angleOutputE AnglePIDANN AnglePID_C)"
 
 proof - 
 
-  from marabou_combined_results[where ?x1.0="normI 1 x_1" and ?x2.0="normI 2 x_2"] have m3: 
+  from marabou_results[where ?x1.0="normI 1 x_1" and ?x2.0="normI 2 x_2"] have m3: 
           "normI 1 x_1 \<ge> normI 1 (inRanges(1).1) \<and> 
           normI 1 x_1 \<le> normI 1 (inRanges(1).2) \<and>
           normI 2 x_2 \<ge> normI 2 (inRanges(2).1) \<and>
@@ -246,27 +248,16 @@ proof -
           normI 1 x_1 \<le> normI 1 (inRanges(1).2) \<and>
           normI 2 x_2 \<ge> normI 2 (inRanges(2).1) \<and>
           normI 2 x_2 \<le> normI 2 (inRanges(2).2) \<and>
-          \<not> annout 2 1 [normI 1 x_1, normI 2 x_2] \<ge> normO 1 ((P * denormI 1 (fst(int(1))) + (D * denormI 2 (fst(int(2)))) ) + \<epsilon>)
-           \<and>
-          \<not> annout 2 1 [normI 1 x_1, normI 2 x_2] \<le> normO 1 ((P * denormI 1 (snd(int(1))) + (D * denormI 2 (snd(int(2)))) ) - \<epsilon>)"
-    by (simp add: int_def)
-
-   have "... = (
-    
-          normI 1 x_1 \<ge> normI 1 (inRanges(1).1) \<and> 
-          normI 1 x_1 \<le> normI 1 (inRanges(1).2) \<and>
-          normI 2 x_2 \<ge> normI 2 (inRanges(2).1) \<and>
-          normI 2 x_2 \<le> normI 2 (inRanges(2).2) \<and>
-     annout 2 1 [normI 1 x_1, normI 2 x_2] \<ge> normO 1 (norm_spec (snd(int(1))) (snd(int(2))) - \<epsilon>)
+     annout 2 1 [normI 1 x_1, normI 2 x_2] \<ge> normO 1 (norm_spec (snd(normRanges(1))) (snd(normRanges(2))) - \<epsilon>)
       \<and> 
-     annout 2 1 [normI 1 x_1, normI 2 x_2] \<le> normO 1 (norm_spec (fst(int(1))) (fst(int(2))) + \<epsilon>)
-    )"
+     annout 2 1 [normI 1 x_1, normI 2 x_2] \<le> normO 1 (norm_spec (fst(normRanges(1))) (fst(normRanges(2))) + \<epsilon>)
+     "
      using nle_le
      unfolding norm_spec_def
-     apply (simp)
-     using m3 by force
+     apply (simp add: normRanges_def)
+     by linarith
   
-  (*Important step, get from the intervals to the actual fixed variables:
+  (*Important step, get from the intervals to the actual variables:
     We can still have this, at the moment, be on the normalised ranges.  *)
    have "... \<longrightarrow>
      annout 2 1 [normI 1 x_1, normI 2 x_2] \<ge> normO 1 (norm_spec (normI 1 x_1) (normI 2 x_2) - \<epsilon>)
@@ -280,19 +271,19 @@ proof -
           normI 1 x_1 \<le> normI 1 (inRanges(1).2) \<and>
           normI 2 x_2 \<ge> normI 2 (inRanges(2).1) \<and>
           normI 2 x_2 \<le> normI 2 (inRanges(2).2) \<and>
-          annout 2 1 [normI 1 x_1, normI 2 x_2] \<ge> normO 1 (norm_spec (snd(int(1))) (snd(int(2))) - \<epsilon>)
+          annout 2 1 [normI 1 x_1, normI 2 x_2] \<ge> normO 1 (norm_spec (snd(normRanges(1))) (snd(normRanges(2))) - \<epsilon>)
       \<and> 
-     annout 2 1 [normI 1 x_1, normI 2 x_2] \<le> normO 1 (norm_spec (fst(int(1))) (fst(int(2))) + \<epsilon>)"
+     annout 2 1 [normI 1 x_1, normI 2 x_2] \<le> normO 1 (norm_spec (fst(normRanges(1))) (fst(normRanges(2))) + \<epsilon>)"
      show "\<forall> x_1 x_2 y_1 y_2. x_1 \<le> y_1 \<and> x_2 \<le> y_2 \<longrightarrow> norm_spec x_1 x_2 \<le> norm_spec y_1 y_2" 
        using assms apply (simp add: norm_spec_mono)
        done
 
-     show "fst (int(1)) \<le> normI 1 x_1 \<and> normI 1 x_1 \<le> snd (int(1))"
-       by (metis \<open>normI 1 (fst (inRanges(1)\<^sub>s)) \<le> normI 1 x_1 \<and> normI 1 x_1 \<le> normI 1 (snd (inRanges(1)\<^sub>s)) \<and> normI 2 (fst (inRanges(2)\<^sub>s)) \<le> normI 2 x_2 \<and> normI 2 x_2 \<le> normI 2 (snd (inRanges(2)\<^sub>s)) \<and> normO 1 (norm_spec (snd (thm2_TEMP.int(1)\<^sub>s)) (snd (thm2_TEMP.int(2)\<^sub>s)) - \<epsilon>) \<le> f_ann (normI 1 x_1) (normI 2 x_2) \<and> f_ann (normI 1 x_1) (normI 2 x_2) \<le> normO 1 (norm_spec (fst (thm2_TEMP.int(1)\<^sub>s)) (fst (thm2_TEMP.int(2)\<^sub>s)) + \<epsilon>)\<close> cancel_comm_monoid_add_class.diff_cancel fst_conv nth_Cons_0 snd_conv thm2_TEMP.int_def)
+     show "fst (normRanges(1)) \<le> normI 1 x_1 \<and> normI 1 x_1 \<le> snd (normRanges(1))"
+       by (metis \<open>normI 1 (fst (inRanges(1)\<^sub>s)) \<le> normI 1 x_1 \<and> normI 1 x_1 \<le> normI 1 (snd (inRanges(1)\<^sub>s)) \<and> normI 2 (fst (inRanges(2)\<^sub>s)) \<le> normI 2 x_2 \<and> normI 2 x_2 \<le> normI 2 (snd (inRanges(2)\<^sub>s)) \<and> normO 1 (norm_spec (snd (thm2_TEMP.normRanges(1)\<^sub>s)) (snd (thm2_TEMP.normRanges(2)\<^sub>s)) - \<epsilon>) \<le> f_ann (normI 1 x_1) (normI 2 x_2) \<and> f_ann (normI 1 x_1) (normI 2 x_2) \<le> normO 1 (norm_spec (fst (thm2_TEMP.normRanges(1)\<^sub>s)) (fst (thm2_TEMP.normRanges(2)\<^sub>s)) + \<epsilon>)\<close> cancel_comm_monoid_add_class.diff_cancel fst_conv nth_Cons_0 snd_conv thm2_TEMP.normRanges_def)
        
 
-     show "fst (int(2)\<^sub>s) \<le> normI 2 x_2  \<and> normI 2 x_2 \<le> snd (int(2)\<^sub>s)"
-       by (metis One_nat_def \<open>normI 1 (fst (inRanges(1)\<^sub>s)) \<le> normI 1 x_1 \<and> normI 1 x_1 \<le> normI 1 (snd (inRanges(1)\<^sub>s)) \<and> normI 2 (fst (inRanges(2)\<^sub>s)) \<le> normI 2 x_2 \<and> normI 2 x_2 \<le> normI 2 (snd (inRanges(2)\<^sub>s)) \<and> normO 1 (norm_spec (snd (thm2_TEMP.int(1)\<^sub>s)) (snd (thm2_TEMP.int(2)\<^sub>s)) - \<epsilon>) \<le> f_ann (normI 1 x_1) (normI 2 x_2) \<and> f_ann (normI 1 x_1) (normI 2 x_2) \<le> normO 1 (norm_spec (fst (thm2_TEMP.int(1)\<^sub>s)) (fst (thm2_TEMP.int(2)\<^sub>s)) + \<epsilon>)\<close> diff_Suc_1 nat_1_add_1 nth_Cons_0 nth_Cons_Suc plus_1_eq_Suc split_pairs thm2_TEMP.int_def)
+     show "fst (normRanges(2)\<^sub>s) \<le> normI 2 x_2  \<and> normI 2 x_2 \<le> snd (normRanges(2)\<^sub>s)"
+       by (metis One_nat_def \<open>normI 1 (fst (inRanges(1)\<^sub>s)) \<le> normI 1 x_1 \<and> normI 1 x_1 \<le> normI 1 (snd (inRanges(1)\<^sub>s)) \<and> normI 2 (fst (inRanges(2)\<^sub>s)) \<le> normI 2 x_2 \<and> normI 2 x_2 \<le> normI 2 (snd (inRanges(2)\<^sub>s)) \<and> normO 1 (norm_spec (snd (thm2_TEMP.normRanges(1)\<^sub>s)) (snd (thm2_TEMP.normRanges(2)\<^sub>s)) - \<epsilon>) \<le> f_ann (normI 1 x_1) (normI 2 x_2) \<and> f_ann (normI 1 x_1) (normI 2 x_2) \<le> normO 1 (norm_spec (fst (thm2_TEMP.normRanges(1)\<^sub>s)) (fst (thm2_TEMP.normRanges(2)\<^sub>s)) + \<epsilon>)\<close> diff_Suc_1 nat_1_add_1 nth_Cons_0 nth_Cons_Suc plus_1_eq_Suc split_pairs thm2_TEMP.normRanges_def)
        
 
      show "0 \<le> \<epsilon>" 
@@ -301,9 +292,9 @@ proof -
      show "fst (outRanges ! 0) < snd (outRanges ! 0) \<and> fst annRange < snd annRange" using assms by simp
         
      show 
-     "f_ann (normI 1 x_1) (normI 2 x_2) \<le> normO 1 (norm_spec (fst (int(1))) (fst (int(2))) + \<epsilon>) \<and>
-      f_ann (normI 1 x_1) (normI 2 x_2) \<ge> normO 1 (norm_spec (snd (int(1))) (snd (thm2_TEMP.int(2))) - \<epsilon>)"
-       using \<open>normI 1 (fst (inRanges(1)\<^sub>s)) \<le> normI 1 x_1 \<and> normI 1 x_1 \<le> normI 1 (snd (inRanges(1)\<^sub>s)) \<and> normI 2 (fst (inRanges(2)\<^sub>s)) \<le> normI 2 x_2 \<and> normI 2 x_2 \<le> normI 2 (snd (inRanges(2)\<^sub>s)) \<and> normO 1 (norm_spec (snd (thm2_TEMP.int(1)\<^sub>s)) (snd (thm2_TEMP.int(2)\<^sub>s)) - \<epsilon>) \<le> f_ann (normI 1 x_1) (normI 2 x_2) \<and> f_ann (normI 1 x_1) (normI 2 x_2) \<le> normO 1 (norm_spec (fst (thm2_TEMP.int(1)\<^sub>s)) (fst (thm2_TEMP.int(2)\<^sub>s)) + \<epsilon>)\<close> by fastforce
+     "f_ann (normI 1 x_1) (normI 2 x_2) \<le> normO 1 (norm_spec (fst (normRanges(1))) (fst (normRanges(2))) + \<epsilon>) \<and>
+      f_ann (normI 1 x_1) (normI 2 x_2) \<ge> normO 1 (norm_spec (snd (normRanges(1))) (snd (thm2_TEMP.normRanges(2))) - \<epsilon>)"
+       using \<open>normI 1 (fst (inRanges(1)\<^sub>s)) \<le> normI 1 x_1 \<and> normI 1 x_1 \<le> normI 1 (snd (inRanges(1)\<^sub>s)) \<and> normI 2 (fst (inRanges(2)\<^sub>s)) \<le> normI 2 x_2 \<and> normI 2 x_2 \<le> normI 2 (snd (inRanges(2)\<^sub>s)) \<and> normO 1 (norm_spec (snd (thm2_TEMP.normRanges(1)\<^sub>s)) (snd (thm2_TEMP.normRanges(2)\<^sub>s)) - \<epsilon>) \<le> f_ann (normI 1 x_1) (normI 2 x_2) \<and> f_ann (normI 1 x_1) (normI 2 x_2) \<le> normO 1 (norm_spec (fst (thm2_TEMP.normRanges(1)\<^sub>s)) (fst (thm2_TEMP.normRanges(2)\<^sub>s)) + \<epsilon>)\<close> by fastforce
        
      qed
 
@@ -348,8 +339,8 @@ proof -
       by (smt (verit) assms(2) mono_normI)
 
     have "y_1 = P * x_1 + D * x_2 \<longrightarrow> \<bar>denormO 1 (f_ann (normI 1 x_1) (normI 2 x_2)) - y_1\<bar> \<le> \<epsilon>"
-      by (metis \<open>(P * denormI 1 (normI 1 x_1) + D * denormI 2 (normI 2 x_2) - \<epsilon> \<le> denormO 1 (f_ann (normI 1 x_1) (normI 2 x_2)) \<and> denormO 1 (f_ann (normI 1 x_1) (normI 2 x_2)) \<le> P * denormI 1 (normI 1 x_1) + D * denormI 2 (normI 2 x_2) + \<epsilon>) = (P * x_1 + D * x_2 - \<epsilon> \<le> denormO 1 (f_ann (normI 1 x_1) (normI 2 x_2)) \<and> denormO 1 (f_ann (normI 1 x_1) (normI 2 x_2)) \<le> P * x_1 + D * x_2 + \<epsilon>)\<close> \<open>(P * x_1 + D * x_2 - \<epsilon> \<le> denormO 1 (f_ann (normI 1 x_1) (normI 2 x_2)) \<and> denormO 1 (f_ann (normI 1 x_1) (normI 2 x_2)) \<le> P * x_1 + D * x_2 + \<epsilon>) = (\<bar>denormO 1 (f_ann (normI 1 x_1) (normI 2 x_2)) - (P * x_1 + D * x_2)\<bar> \<le> \<epsilon>)\<close> \<open>(denormO 1 (normO 1 (P * denormI 1 (normI 1 x_1) + D * denormI 2 (normI 2 x_2) - \<epsilon>)) \<le> denormO 1 (f_ann (normI 1 x_1) (normI 2 x_2)) \<and> denormO 1 (f_ann (normI 1 x_1) (normI 2 x_2)) \<le> denormO 1 (normO 1 (P * denormI 1 (normI 1 x_1) + D * denormI 2 (normI 2 x_2) + \<epsilon>))) = (P * denormI 1 (normI 1 x_1) + D * denormI 2 (normI 2 x_2) - \<epsilon> \<le> denormO 1 (f_ann (normI 1 x_1) (normI 2 x_2)) \<and> denormO 1 (f_ann (normI 1 x_1) (normI 2 x_2)) \<le> P * denormI 1 (normI 1 x_1) + D * denormI 2 (normI 2 x_2) + \<epsilon>)\<close> \<open>(normO 1 (P * denormI 1 (normI 1 x_1) + D * denormI 2 (normI 2 x_2) - \<epsilon>) \<le> f_ann (normI 1 x_1) (normI 2 x_2) \<and> f_ann (normI 1 x_1) (normI 2 x_2) \<le> normO 1 (P * denormI 1 (normI 1 x_1) + D * denormI 2 (normI 2 x_2) + \<epsilon>)) = (denormO 1 (normO 1 (P * denormI 1 (normI 1 x_1) + D * denormI 2 (normI 2 x_2) - \<epsilon>)) \<le> denormO 1 (f_ann (normI 1 x_1) (normI 2 x_2)) \<and> denormO 1 (f_ann (normI 1 x_1) (normI 2 x_2)) \<le> denormO 1 (normO 1 (P * denormI 1 (normI 1 x_1) + D * denormI 2 (normI 2 x_2) + \<epsilon>)))\<close> \<open>normI 1 (fst (inRanges(1)\<^sub>s)) \<le> normI 1 x_1 \<and> normI 1 x_1 \<le> normI 1 (snd (inRanges(1)\<^sub>s)) \<and> normI 2 (fst (inRanges(2)\<^sub>s)) \<le> normI 2 x_2 \<and> normI 2 x_2 \<le> normI 2 (snd (inRanges(2)\<^sub>s)) \<and> normO 1 (norm_spec (snd (thm2_TEMP.int(1)\<^sub>s)) (snd (thm2_TEMP.int(2)\<^sub>s)) - \<epsilon>) \<le> f_ann (normI 1 x_1) (normI 2 x_2) \<and> f_ann (normI 1 x_1) (normI 2 x_2) \<le> normO 1 (norm_spec (fst (thm2_TEMP.int(1)\<^sub>s)) (fst (thm2_TEMP.int(2)\<^sub>s)) + \<epsilon>) \<longrightarrow> normO 1 (norm_spec (normI 1 x_1) (normI 2 x_2) - \<epsilon>) \<le> f_ann (normI 1 x_1) (normI 2 x_2) \<and> f_ann (normI 1 x_1) (normI 2 x_2) \<le> normO 1 (norm_spec (normI 1 x_1) (normI 2 x_2) + \<epsilon>)\<close> goal3 linorder_linear m3 norm_spec_def)
-
+      by (metis \<open>(P * denormI 1 (normI 1 x_1) + D * denormI 2 (normI 2 x_2) - \<epsilon> \<le> denormO 1 (f_ann (normI 1 x_1) (normI 2 x_2)) \<and> denormO 1 (f_ann (normI 1 x_1) (normI 2 x_2)) \<le> P * denormI 1 (normI 1 x_1) + D * denormI 2 (normI 2 x_2) + \<epsilon>) = (P * x_1 + D * x_2 - \<epsilon> \<le> denormO 1 (f_ann (normI 1 x_1) (normI 2 x_2)) \<and> denormO 1 (f_ann (normI 1 x_1) (normI 2 x_2)) \<le> P * x_1 + D * x_2 + \<epsilon>)\<close> \<open>(P * x_1 + D * x_2 - \<epsilon> \<le> denormO 1 (f_ann (normI 1 x_1) (normI 2 x_2)) \<and> denormO 1 (f_ann (normI 1 x_1) (normI 2 x_2)) \<le> P * x_1 + D * x_2 + \<epsilon>) = (\<bar>denormO 1 (f_ann (normI 1 x_1) (normI 2 x_2)) - (P * x_1 + D * x_2)\<bar> \<le> \<epsilon>)\<close> \<open>(denormO 1 (normO 1 (P * denormI 1 (normI 1 x_1) + D * denormI 2 (normI 2 x_2) - \<epsilon>)) \<le> denormO 1 (f_ann (normI 1 x_1) (normI 2 x_2)) \<and> denormO 1 (f_ann (normI 1 x_1) (normI 2 x_2)) \<le> denormO 1 (normO 1 (P * denormI 1 (normI 1 x_1) + D * denormI 2 (normI 2 x_2) + \<epsilon>))) = (P * denormI 1 (normI 1 x_1) + D * denormI 2 (normI 2 x_2) - \<epsilon> \<le> denormO 1 (f_ann (normI 1 x_1) (normI 2 x_2)) \<and> denormO 1 (f_ann (normI 1 x_1) (normI 2 x_2)) \<le> P * denormI 1 (normI 1 x_1) + D * denormI 2 (normI 2 x_2) + \<epsilon>)\<close> \<open>(normO 1 (P * denormI 1 (normI 1 x_1) + D * denormI 2 (normI 2 x_2) - \<epsilon>) \<le> f_ann (normI 1 x_1) (normI 2 x_2) \<and> f_ann (normI 1 x_1) (normI 2 x_2) \<le> normO 1 (P * denormI 1 (normI 1 x_1) + D * denormI 2 (normI 2 x_2) + \<epsilon>)) = (denormO 1 (normO 1 (P * denormI 1 (normI 1 x_1) + D * denormI 2 (normI 2 x_2) - \<epsilon>)) \<le> denormO 1 (f_ann (normI 1 x_1) (normI 2 x_2)) \<and> denormO 1 (f_ann (normI 1 x_1) (normI 2 x_2)) \<le> denormO 1 (normO 1 (P * denormI 1 (normI 1 x_1) + D * denormI 2 (normI 2 x_2) + \<epsilon>)))\<close> \<open>normI 1 (fst (inRanges(1)\<^sub>s)) \<le> normI 1 x_1 \<and> normI 1 x_1 \<le> normI 1 (snd (inRanges(1)\<^sub>s)) \<and> normI 2 (fst (inRanges(2)\<^sub>s)) \<le> normI 2 x_2 \<and> normI 2 x_2 \<le> normI 2 (snd (inRanges(2)\<^sub>s)) \<and> normO 1 (norm_spec (snd (normRanges(1)\<^sub>s)) (snd (normRanges(2)\<^sub>s)) - \<epsilon>) \<le> f_ann (normI 1 x_1) (normI 2 x_2) \<and> f_ann (normI 1 x_1) (normI 2 x_2) \<le> normO 1 (norm_spec (fst (normRanges(1)\<^sub>s)) (fst (normRanges(2)\<^sub>s)) + \<epsilon>) \<longrightarrow> normO 1 (norm_spec (normI 1 x_1) (normI 2 x_2) - \<epsilon>) \<le> f_ann (normI 1 x_1) (normI 2 x_2) \<and> f_ann (normI 1 x_1) (normI 2 x_2) \<le> normO 1 (norm_spec (normI 1 x_1) (normI 2 x_2) + \<epsilon>)\<close> goal3 m3 norm_spec_def)
+      
     thus "?thesis" 
       using assms(1) conf_vcs by (auto)
 
